src/Bedrock/Proofs/Expr.v
@@ -1,11 +1,21 @@
 Require Import Coq.ZArith.ZArith.
 Require Import Coq.Lists.List.
+Require Import Coq.micromega.Lia.
 Require Import bedrock2.Syntax.
+Require Import bedrock2.WeakestPreconditionProperties.
+Require Import coqutil.Word.Interface coqutil.Word.Properties.
+Require Import coqutil.Map.Interface.
+Require Import Crypto.CastLemmas.
 Require Import Crypto.Bedrock.Types.
+Require Import Crypto.Bedrock.Tactics.
+Require Import Crypto.Bedrock.Util.
 Require Import Crypto.Bedrock.Proofs.Varnames.
 Require Import Crypto.Bedrock.Translation.Expr.
 Require Import Crypto.Language.API.
+Require Import Rewriter.Util.Bool.Reflect.
 Require Import Crypto.Util.ZRange.
+Require Import Crypto.Util.Tactics.BreakMatch.
+Require Import Crypto.Util.ZUtil.Tactics.LtbToLt.
 Local Open Scope Z_scope.
 
 Import API.Compilers.
@@ -51,51 +61,165 @@ Section Expr.
                                       (expr.Ident (ident.Literal (t:=base.type.zrange) r1)))
                                    (expr.Ident (ident.Literal (t:=base.type.zrange) r2)))) x)
   | valid_fst :
-      forall rc (x y : API.expr type_Z),
+      forall (x : API.expr type_ZZ),
         valid_expr true x ->
-        valid_expr rc
-                   (expr.App (expr.Ident ident.fst)
-                             (expr.App (expr.App (expr.Ident ident.pair) x) y))
+        valid_expr false (expr.App (expr.Ident ident.fst) x)
   | valid_snd :
-      forall rc (x y : API.expr type_Z),
-        valid_expr true y ->
-        valid_expr rc
-                   (expr.App (expr.Ident ident.snd)
-                             (expr.App (expr.App (expr.Ident ident.pair) x) y))
+      forall (x : API.expr type_ZZ),
+        valid_expr true x ->
+        valid_expr false (expr.App (expr.Ident ident.fst) x)
   | valid_literalz :
       forall rc z,
-        (* either bounded or casts not required *)
-        (is_bounded_by_bool z max_range || negb rc = true)%bool ->
+        is_bounded_by_bool z max_range = true ->
         valid_expr rc (expr.Ident (ident.Literal (t:=base.type.Z) z))
+  | valid_var :
+      forall v, valid_expr (t:=base_Z) false (expr.Var v)
   | valid_nth_default :
-      forall rc d l i,
+      forall d l i,
         valid_expr true d ->
         valid_expr
-          rc (* casts not required, since a list of vars must be already cast *)
+          false
           (expr.App (expr.App (expr.App (expr.Ident ident.List_nth_default) d)
                               (expr.Var (t:=type_listZ) l))
                     (expr.Ident (ident.Literal i)))
-  | valid_var :
-      forall rc t v, valid_expr (t:= t) rc (expr.Var v)
+  | valid_shiftr :
+      forall (x : API.expr type_Z) n,
+        valid_expr true x ->
+        0 <= n < Semantics.width ->
+        valid_expr (t:=base_Z) false
+                   (expr.App (expr.App (expr.Ident ident.Z_shiftr) x)
+                   (expr.Ident (ident.Literal (t:=base.type.Z) n)))
   | valid_basic_binop :
-      forall rc i (x y : API.expr type_Z),
+      forall i (x y : API.expr type_Z),
         translate_binop i <> None ->
         valid_expr true x ->
         valid_expr true y ->
-        valid_expr (t:=base_Z) rc (expr.App (expr.App (expr.Ident i) x) y)
+        valid_expr (t:=base_Z) false (expr.App (expr.App (expr.Ident i) x) y)
   | valid_truncating_binop :
-      forall rc i (s : Z) (x y : API.expr type_Z),
-        translate_truncating_binop i <> None ->
-        s = Semantics.width ->
+      forall i (s : Z) (x y : API.expr type_Z),
+        translate_truncating_binop i s <> None ->
         valid_expr true x ->
         valid_expr true y ->
-        valid_expr (t:=base_Z) rc
+        valid_expr (t:=base_Z) false
                    (expr.App (expr.App
                                 (expr.App (expr.Ident i)
                                           (expr.Ident (ident.Literal (t:=base.type.Z) s)))
                                 x) y)
   .
 
+  Lemma equivalent_cast1 r x y locals:
+    range_good r = true ->
+    locally_equivalent (t:=base_Z) x y locals ->
+    locally_equivalent (t:=base_Z) (ident.cast (ident.literal r) x) y locals.
+  Proof.
+    cbv [range_good max_range]. cbn [locally_equivalent equivalent rep.equiv rep.Z].
+    let X := fresh in
+    assert (0 <= Semantics.width) as X by (pose proof word.width_pos; lia);
+      pose proof (Z.pow_pos_nonneg 2 Semantics.width ltac:(lia) X).
+    intros; progress reflect_beq_to_eq zrange_beq; subst r.
+    sepsimpl.
+    cbv [ident.literal WeakestPrecondition.dexpr] in *.
+    eapply Proper_expr; [ | eassumption ].
+    repeat intro; subst. apply word.of_Z_inj_mod.
+    rewrite ident.cast_out_of_bounds_simple_0_mod by lia.
+    rewrite Z.sub_simpl_r, Z.mod_mod by lia.
+    reflexivity.
+  Qed.
+
+  Lemma equivalent_cast2 r1 r2 x y locals :
+    range_good r1 = true ->
+    range_good r2 = true ->
+    locally_equivalent (t:=base_ZZ) x y locals ->
+    locally_equivalent (t:=base_ZZ)
+                       (ident.cast2 (ident.literal r1, ident.literal r2) x) y locals.
+  Proof.
+    cbv [range_good max_range]. cbn [locally_equivalent equivalent rep.equiv rep.Z ].
+    let X := fresh in
+    assert (0 <= Semantics.width) as X by (pose proof word.width_pos; lia);
+      pose proof (Z.pow_pos_nonneg 2 Semantics.width ltac:(lia) X).
+    intros; progress reflect_beq_to_eq zrange_beq; subst r1 r2.
+    cbv [ident.cast2 ident.literal WeakestPrecondition.dexpr] in *.
+    sepsimpl.
+    all:eapply Proper_expr; [ | eassumption ].
+    all:repeat intro; subst; apply word.of_Z_inj_mod.
+    all:rewrite ident.cast_out_of_bounds_simple_0_mod by lia.
+    all:rewrite Z.sub_simpl_r, Z.mod_mod by lia.
+    all:reflexivity.
+  Qed.
+
+  (*
+  (* version generalized to any t, necessary to destruct i *)
+  Lemma translate_binop_correct' {t} :
+    forall (i : ident.ident t)
+           (xs : type.for_each_lhs_of_arrow API.interp_type t)
+           (ys : type.for_each_lhs_of_arrow rtype t)
+           op locals,
+      translate_binop i = Some op ->
+      locally_equivalent_args xs ys locals ->
+      let rhs : type.for_each_lhs_of_arrow rtype t -> base_rtype (type.final_codomain t)
+          := match t as t0 return
+                   type.for_each_lhs_of_arrow rtype t0 ->
+                   base_rtype (type.final_codomain t0) with
+             | (type_Z -> type_Z -> type_Z)%etype =>
+               fun (y : (Syntax.expr * (Syntax.expr * unit))) =>
+                 let y1 := fst y in
+                 let y2 := fst (snd y) in
+                 expr.op op y1 y2
+             | _ => fun _ => base_rtype_of_ltype (dummy_base_ltype _)
+             end in
+      locally_equivalent (type.app_curried (Compilers.ident_interp i) xs) 
+                         (rhs ys) locals.
+  Proof.
+    cbv [translate_binop]; intros *.
+    break_match; try congruence; intros.
+    all:repeat match goal with
+               | _ => progress sepsimpl
+               | _ => progress cbn [fst snd
+                                        Compilers.ident_interp
+                                        type.app_curried
+                                        type.final_codomain
+                                        locally_equivalent
+                                        equivalent rep.Z rep.equiv
+                                        equivalent_args
+                                        Semantics.interp_binop
+                                        locally_equivalent_args] in *
+               | _ => progress
+                        (cbv [WeakestPrecondition.dexpr] in *;
+                         cbn [WeakestPrecondition.expr WeakestPrecondition.expr_body])
+               | H : Some _ = Some _ |- _ => inversion H; subst; clear H
+               end.
+    all: (do 2 (eapply Proper_expr; [ | eassumption]; repeat intro; subst)).
+    all:autorewrite with rew_word_morphism; try reflexivity.
+      
+    { apply word.unsigned_inj.
+      rewrite word.unsigned_and.
+      rewrite !word.unsigned_of_Z.
+      Search word.and.
+    
+
+  Lemma translate_binop_correct
+        (i : ident.ident (type_Z -> type_Z -> type_Z))
+        (x1 x2 : base.interp base_Z)
+        (y1 y2 : Syntax.expr)
+        op locals :
+    translate_binop i = Some op ->
+    locally_equivalent (t:=base_Z) x1 y1 locals ->
+    locally_equivalent (t:=base_Z) x2 y2 locals ->
+    locally_equivalent (Compilers.ident_interp i x1 x2) 
+                       (expr.op op y1 y2) locals.
+  Proof.
+    intros.
+    let H := fresh in
+    pose proof (translate_binop_correct'
+                  i (x1, (x2, tt)) (y1, (y2, tt))) as H;
+      apply H; clear H; eauto; [ ].
+    cbn [locally_equivalent_args equivalent_args fst snd].
+    cbv [locally_equivalent] in *.
+    eapply sep_empty_iff.
+    sepsimpl; eauto.
+  Qed.
+
+  Qed.*)
   Lemma translate_expr_correct {t}
         (* three exprs, representing the same Expr with different vars *)
         (e1 : @API.expr (fun _ => unit) (type.base t))
@@ -109,5 +233,116 @@ Section Expr.
       let out := translate_expr require_cast e3 in
       context_equiv G locals ->
       locally_equivalent (API.interp e2) out locals.
-  Admitted.
+  Proof.
+    cbv zeta.
+    induction 1; inversion 1; cleanup_wf; intros.
+
+    all:repeat match goal with
+               | _ => progress cleanup_wf
+               | H : wf3 _ ?x ?y _ |- _ =>
+                 (* for specific cases, repeatedly do inversion *)
+                 progress match y with
+                          | expr.App _ _ => idtac (* don't invert original, already-inverted hypothesis *)
+                          | _ => match x with
+                                 | context [expr.Ident] =>
+                                   inversion H; clear H
+                                 | context [expr.Var] =>
+                                   inversion H; clear H
+                                 end
+                          end
+               end.
+    { (* cast1 *)
+      cbn [translate_expr has_casts expr.interp Compilers.ident_interp].
+      match goal with H : range_good _ = true |- _ =>
+                      rewrite H end.
+      cbn [negb]; rewrite Bool.andb_false_r.
+      eauto using equivalent_cast1. }
+    { (* cast2 *)
+      cbn [translate_expr has_casts expr.interp Compilers.ident_interp].
+      repeat match goal with H : range_good _ = true |- _ =>
+                             rewrite H end.
+      cbn [negb andb]; rewrite Bool.andb_false_r.
+      eauto using equivalent_cast2. }
+    { (* fst *)
+      cbn [translate_expr has_casts expr.interp Compilers.ident_interp].
+      cbn [negb]. rewrite !Bool.andb_true_r.
+      specialize (IHvalid_expr _ _ _ _ ltac:(eassumption) ltac:(eassumption)).
+      cbn [locally_equivalent equivalent rep.equiv rep.Z] in *.
+      sepsimpl. eauto. }
+    { (* snd *)
+      cbn [translate_expr has_casts expr.interp Compilers.ident_interp].
+      cbn [negb]. rewrite !Bool.andb_true_r.
+      specialize (IHvalid_expr _ _ _ _ ltac:(eassumption) ltac:(eassumption)).
+      cbn [locally_equivalent equivalent rep.equiv rep.Z] in *.
+      sepsimpl. eauto. }
+    { (* literal *)
+      cbn [translate_expr has_casts expr.interp Compilers.ident_interp].
+      repeat match goal with H : is_bounded_by_bool _ _ = true |- _ =>
+                             rewrite H end.
+      cbn [negb]. rewrite !Bool.andb_false_r.
+      cbn [locally_equivalent equivalent rep.equiv rep.Z].
+      sepsimpl. reflexivity. }
+    { (* var *)
+      cbn [translate_expr has_casts expr.interp Compilers.ident_interp].
+      cbn [negb]. rewrite !Bool.andb_true_r.
+      match goal with
+      | H : context_equiv _ _ |- _ =>
+        cbv [context_equiv] in H;
+          rewrite Forall_forall in H;
+          specialize (H _ ltac:(eassumption))
+      end.
+      eauto. }
+    { (* nth_default *)
+      cbn [translate_expr has_casts expr.interp Compilers.ident_interp].
+      cbn [negb]. rewrite !Bool.andb_true_r.
+      cbv [ident.literal].
+      match goal with
+        |- locally_equivalent (nth_default ?d1 ?l1 ?i) (nth_default ?d2 ?l2 ?i) ?locals =>
+        let R := constr:(fun x y => locally_equivalent (t:=base_Z) x y locals) in
+        assert (length l1 = length l2 /\
+                (forall i,
+                    R (nth_default d1 l1 i) (nth_default d2 l2 i)));
+          [ apply (@Forall.Forall2_forall_iff'' _ _ R) | cleanup; solve [eauto] ]
+      end.
+      split; [ | solve [eauto] ].
+      match goal with
+      | H : context_equiv _ _ |- _ =>
+        cbv [context_equiv] in H;
+          rewrite Forall_forall in H;
+          specialize (H _ ltac:(eassumption))
+      end.
+      eauto. }
+    { (* shiftr *) 
+      cbn [translate_expr has_casts expr.interp Compilers.ident_interp].
+      cbn [negb]. rewrite !Bool.andb_true_r.
+      specialize (IHvalid_expr _ _ _ _ ltac:(eassumption) ltac:(eassumption)).
+      cbv [is_bounded_by_bool]. cbn [upper lower].
+      break_match;
+        try match goal with
+            | H : (_ && _)%bool = true |- _ =>
+              apply Bool.andb_true_iff in H; cleanup
+            | H : (_ && _)%bool = false |- _ =>
+              apply Bool.andb_false_iff in H; destruct H
+            end; Z.ltb_to_lt; try lia; [ ].
+      cbn [locally_equivalent equivalent rep.equiv rep.Z ident.literal] in *.
+      cbv [WeakestPrecondition.dexpr] in *.
+      cbn [WeakestPrecondition.expr WeakestPrecondition.expr_body
+                                    Semantics.interp_binop].
+      sepsimpl. eapply Proper_expr; [ | eassumption ].
+      repeat intro; subst.
+      cbv [WeakestPrecondition.literal dlet.dlet ident.literal].
+      apply word.unsigned_inj.
+      rewrite word.unsigned_sru, !word.unsigned_of_Z.
+      (* need a proof that says if valid_expr true, then bounded. Or maybe if in
+         context, then bounded *)
+      all:admit. }
+    { (* basic binop *)
+      (* GROSS -- shiftr special case vomits all over this *)
+      cbn [translate_expr has_casts expr.interp Compilers.ident_interp].
+      cbn [negb]. rewrite !Bool.andb_true_r.
+      break_match.
+      break_match; try congruence; [ ].
+      apply translate_binop_correct; eauto. }
+
+  Qed.
 End Expr.
